o Added sequences to second order terms.

terms/sovar.v
@@ -1,6 +1,8 @@
 (*
 
   Copyright 2014 Cornell University
+  Copyright 2015 Cornell University
+  Copyright 2016 Cornell University
 
   This file is part of VPrl (the Verified Nuprl project).
 
@@ -18,7 +20,10 @@
   along with VPrl.  If not, see <http://www.gnu.org/licenses/>.
 
 
-  Website: http://nuprl.org/html/verification/
+  Websites: http://nuprl.org/html/verification/
+            http://nuprl.org/html/Nuprl2Coq
+            https://github.com/vrahli/NuprlInCoq
+
   Authors: Abhishek Anand & Vincent Rahli
 
 *)
@@ -37,6 +42,7 @@ Require Export terms_apply.
  *)
 Inductive SOTerm {o} : tuniv :=
 | sovar : NVar -> list SOTerm -> SOTerm
+| soseq : (nat -> @NTerm o) -> SOTerm
 | soterm : @Opid o -> list SOBTerm -> SOTerm
 with SOBTerm {o} : tuniv :=
 | sobterm : list NVar -> SOTerm -> SOBTerm.
@@ -45,6 +51,7 @@ with SOBTerm {o} : tuniv :=
 Definition mk_soaxiom {o} : @SOTerm o := soterm (Can NAxiom) [].
 
 
+(*
 (**
 
   true if the [SOTerm] is a [NTerm]
@@ -60,6 +67,7 @@ with is_bterm {o} (bt : @SOBTerm o) : bool :=
        match bt with
          | sobterm _ t => is_nterm t
        end.
+*)
 
 (**
 
@@ -69,12 +77,24 @@ with is_bterm {o} (bt : @SOBTerm o) : bool :=
  *)
 Fixpoint soterm2nterm {o} (t : @SOTerm o) : @NTerm o :=
   match t with
-    | sovar v ts => apply_list (mk_var v) (map soterm2nterm ts)
-    | soterm opid bs => oterm opid (map sobterm2bterm bs)
+  | sovar v ts => apply_list (mk_var v) (map soterm2nterm ts)
+  | soseq s => sterm s
+  | soterm opid bs => oterm opid (map sobterm2bterm bs)
   end
 with sobterm2bterm {o} (bt : @SOBTerm o) : @BTerm o :=
        match bt with
          | sobterm vs t => bterm vs (soterm2nterm t)
+       end.
+
+Fixpoint nterm2soterm {o} (t : @NTerm o) : @SOTerm o :=
+  match t with
+  | vterm v => sovar v []
+  | sterm s => soseq s
+  | oterm opid bs => soterm opid (map bterm2sobterm bs)
+  end
+with bterm2sobterm {o} (bt : @BTerm o) : @SOBTerm o :=
+       match bt with
+       | bterm vs t => sobterm vs (nterm2soterm t)
        end.
 
 Definition sovar_sig := NVar # nat.
@@ -203,8 +223,9 @@ Definition vars2sovars := map var2sovar.
 
 Fixpoint so_free_vars {o} (t : @SOTerm o) : list sovar_sig :=
   match t with
-    | sovar v ts => (v,length ts) :: (flat_map so_free_vars ts)
-    | soterm op bs => flat_map so_free_vars_bterm bs
+  | sovar v ts => (v,length ts) :: (flat_map so_free_vars ts)
+  | soseq s => []
+  | soterm op bs => flat_map so_free_vars_bterm bs
   end
 with so_free_vars_bterm {o} (bt : @SOBTerm o) : list sovar_sig :=
        match bt with
@@ -216,8 +237,9 @@ with so_free_vars_bterm {o} (bt : @SOBTerm o) : list sovar_sig :=
 
 Fixpoint all_fo_vars {o} (t : @SOTerm o) : list NVar :=
   match t with
-    | sovar v ts => v :: flat_map all_fo_vars ts
-    | soterm op bs => flat_map all_fo_vars_bterm bs
+  | sovar v ts => v :: flat_map all_fo_vars ts
+  | soseq s => []
+  | soterm op bs => flat_map all_fo_vars_bterm bs
   end
 with all_fo_vars_bterm {o} (bt : @SOBTerm o) : list NVar :=
        match bt with
@@ -226,8 +248,9 @@ with all_fo_vars_bterm {o} (bt : @SOBTerm o) : list NVar :=
 
 Fixpoint fo_bound_vars {p} (t : @SOTerm p) : list NVar :=
   match t with
-    | sovar _ ts => flat_map fo_bound_vars ts
-    | soterm op bs => flat_map fo_bound_vars_bterm bs
+  | sovar _ ts => flat_map fo_bound_vars ts
+  | soseq _ => []
+  | soterm op bs => flat_map fo_bound_vars_bterm bs
   end
 with fo_bound_vars_bterm {p} (bt : @SOBTerm p) : list NVar :=
        match bt with
@@ -347,17 +370,18 @@ Fixpoint lift_list_option {T} (l : list (option T)) : option (list T) :=
  * be disjoint from all the vars of t *)
 Fixpoint sosub_aux {o} (sub : @SOSub o) (t : SOTerm) : NTerm :=
   match t with
-    | sovar var ts =>
-      match sosub_find sub (var,length ts) with
-        | Some (sosk vs u) => lsubst_aux u (combine vs (map (sosub_aux sub) ts))
-        | None => apply_list (mk_var var) (map (sosub_aux sub) ts)
-      end
-    | soterm opid bts => oterm opid (map (sosub_b_aux sub) bts)
+  | sovar var ts =>
+    match sosub_find sub (var,length ts) with
+    | Some (sosk vs u) => lsubst_aux u (combine vs (map (sosub_aux sub) ts))
+    | None => apply_list (mk_var var) (map (sosub_aux sub) ts)
+    end
+  | soseq s => sterm s
+  | soterm opid bts => oterm opid (map (sosub_b_aux sub) bts)
   end
 with sosub_b_aux {o} (sub : @SOSub o) (bt : SOBTerm) : BTerm :=
        match bt with
-         | sobterm vs t =>
-           bterm vs (sosub_aux (sosub_filter sub (vars2sovars vs)) t)
+       | sobterm vs t =>
+         bterm vs (sosub_aux (sosub_filter sub (vars2sovars vs)) t)
        end.
 
 Definition free_vars_sk {o} (sk : @sosub_kind o) : list NVar :=
@@ -523,33 +547,35 @@ Qed.
 
 Fixpoint fo_change_bvars_alpha {p} (disj : list NVar) (ren : foren) (t : @SOTerm p) :=
   match t with
-    | sovar v ts =>
-      if bnull ts
-      then sovar (rename_var ren v) []
-      else sovar v (map (fo_change_bvars_alpha disj ren) ts)
-    | soterm o bs => soterm o (map (fo_change_bvars_alphabt disj ren) bs)
+  | sovar v ts =>
+    if bnull ts
+    then sovar (rename_var ren v) []
+    else sovar v (map (fo_change_bvars_alpha disj ren) ts)
+  | soseq s => soseq s
+  | soterm o bs => soterm o (map (fo_change_bvars_alphabt disj ren) bs)
   end
 with fo_change_bvars_alphabt {p} disj ren bt :=
        match bt with
-         | sobterm vs t =>
-           let vs' := fresh_distinct_vars (length vs) (vs ++ disj ++ all_fo_vars t ++ foren_vars ren) in
-           sobterm vs' (fo_change_bvars_alpha disj (mk_foren vs vs' ++ ren) t)
+       | sobterm vs t =>
+         let vs' := fresh_distinct_vars (length vs) (vs ++ disj ++ all_fo_vars t ++ foren_vars ren) in
+         sobterm vs' (fo_change_bvars_alpha disj (mk_foren vs vs' ++ ren) t)
        end.
 (* vs in the list of distinct vars above is not necessary but useful *)
 
 Fixpoint so_change_bvars_alpha {p} (disj : list NVar) (ren : soren) (t : @SOTerm p) :=
   match t with
-    | sovar v ts =>
-      sovar
-        (sovar2var (rename_sovar ren (v,length ts)))
-        (map (so_change_bvars_alpha disj ren) ts)
-    | soterm o bs => soterm o (map (so_change_bvars_alphabt disj ren) bs)
+  | sovar v ts =>
+    sovar
+      (sovar2var (rename_sovar ren (v,length ts)))
+      (map (so_change_bvars_alpha disj ren) ts)
+  | soseq s => soseq s
+  | soterm o bs => soterm o (map (so_change_bvars_alphabt disj ren) bs)
   end
 with so_change_bvars_alphabt {p} disj ren bt :=
        match bt with
-         | sobterm vs t =>
-           let vs' := fresh_distinct_vars (length vs) (disj ++ all_fo_vars t ++ soren_vars ren) in
-           sobterm vs' (so_change_bvars_alpha disj (mk_soren (vars2sovars vs) vs' ++ ren) t)
+       | sobterm vs t =>
+         let vs' := fresh_distinct_vars (length vs) (disj ++ all_fo_vars t ++ soren_vars ren) in
+         sobterm vs' (so_change_bvars_alpha disj (mk_soren (vars2sovars vs) vs' ++ ren) t)
        end.
 (* all_fo_vars could just be the free vars above *)
 
@@ -991,8 +1017,9 @@ Fixpoint get_fo_vars (l : list sovar_sig) : list NVar :=
 
 Fixpoint sosize {p} (t : @SOTerm p) : nat :=
   match t with
-    | sovar _ ts => S (addl (map sosize ts))
-    | soterm op bs => S (addl (map sosize_bterm bs))
+  | sovar _ ts => S (addl (map sosize ts))
+  | soseq s => 0
+  | soterm op bs => S (addl (map sosize_bterm bs))
   end
 with sosize_bterm {p} (b : SOBTerm) :=
        match b with
@@ -1022,6 +1049,7 @@ Lemma SOTerm_better_ind2 {p} :
     (forall v ts,
        (forall t, LIn t ts -> P t)
        -> P (sovar v ts))
+    -> (forall s, P (soseq s))
     -> (forall (o : Opid) (bs : list SOBTerm),
           (forall (t t': SOTerm) (vs : list NVar),
              (LIn (sobterm vs t) bs)
@@ -1032,7 +1060,7 @@ Lemma SOTerm_better_ind2 {p} :
        )
     -> forall t : SOTerm, P t.
 Proof.
-  intros P Hvar Hbt.
+  intros P Hvar Hseq Hbt.
   assert (forall n t, sosize t = n -> P t)
     as Hass;
     [ | intros; apply Hass with (n := sosize t); eauto; fail ].
@@ -1045,6 +1073,7 @@ Proof.
     destruct n; cpx.
     pose proof (Hind (sosize t)) as k; autodimp k hyp.
     apply sosize_in in i; omega.
+  - apply Hseq.
   - apply Hbt.
     introv Hin Hs.
     apply Hind with (m := sosize t'); auto.
@@ -1057,37 +1086,46 @@ Lemma SOTerm_better_ind {p} :
     (forall v ts,
        (forall t, LIn t ts -> P t)
        -> P (sovar v ts))
+    -> (forall s, P (soseq s))
     -> (forall (o : Opid) (bs : list SOBTerm),
           (forall t vs, LIn (sobterm vs t) bs -> P t)
           -> P (soterm o bs)
        )
     -> forall t : SOTerm, P t.
 Proof.
-  introv Hv Hind. apply SOTerm_better_ind2; auto.
-  introv Hx. apply Hind. introv Hin. eapply Hx in Hin; eauto.
+  introv Hv Hseq Hind.
+  apply SOTerm_better_ind2; auto.
+  introv Hx.
+  apply Hind.
+  introv Hin.
+  eapply Hx in Hin; eauto.
 Qed.
 
 Tactic Notation "soterm_ind" ident(h) ident(c) :=
   induction h using SOTerm_better_ind;
   [ Case_aux c "sovar"
+  | Case_aux c "soseq"
   | Case_aux c "soterm"
   ].
 
 Tactic Notation "soterm_ind" ident(h) "as" simple_intropattern(I)  ident(c) :=
   induction h as I using SOTerm_better_ind;
   [ Case_aux c "sovar"
+  | Case_aux c "soseq"
   | Case_aux c "soterm"
   ].
 
 Tactic Notation "soterm_ind1" ident(h) "as" simple_intropattern(I)  ident(c) :=
   induction h as I using SOTerm_better_ind;
   [ Case_aux c "sovar"
+  | Case_aux c "soseq"
   | Case_aux c "soterm"
   ].
 
 Tactic Notation "soterm_ind1s" ident(h) "as" simple_intropattern(I)  ident(c) :=
   induction h as I using SOTerm_better_ind2;
   [ Case_aux c "sovar"
+  | Case_aux c "soseq"
   | Case_aux c "soterm"
   ].
 
@@ -1307,7 +1345,7 @@ Lemma so_free_vars_in_all_fo_vars {o} :
   forall (t : @SOTerm o) v n,
     LIn (v, n) (so_free_vars t) -> LIn v (all_fo_vars t).
 Proof.
-  soterm_ind t as [ v ts ind | op lbt ind ] Case; simpl; introv i.
+  soterm_ind t as [ v ts ind |  | op lbt ind ] Case; simpl; introv i; tcsp.
 
   - Case "sovar".
     dorn i; cpx.
@@ -1474,7 +1512,7 @@ Lemma isprogram_sosub_aux_wf {p} :
     -> sosub_wf sub
     -> wf_term (sosub_aux sub t).
 Proof.
-  soterm_ind t as [ v ts ind | o lbt ind ] Case; simpl; introv wft wfs.
+  soterm_ind t as [ v ts ind | | o lbt ind ] Case; simpl; introv wft wfs; tcsp.
 
   - Case "sovar".
     remember (sosub_find sub (v, length ts)) as o;
@@ -1530,7 +1568,7 @@ Lemma isprogram_sosub_aux_free_vars {p} :
       (sovars2vars (remove_so_vars (sodom sub) (so_free_vars t))
                    ++ free_vars_sosub sub).
 Proof.
-  soterm_ind t as [ v ts ind | o lbt ind ] Case; simpl; introv.
+  soterm_ind t as [ v ts ind | | o lbt ind ] Case; simpl; introv; tcsp.
 
   - Case "sovar".
     remember (sosub_find sub (v, length ts)) as o;
@@ -1766,7 +1804,7 @@ Lemma wf_soterm_fo_change_bvars_alpha {o} :
   forall (t : @SOTerm o) disj ren,
     wf_soterm t <=> wf_soterm (fo_change_bvars_alpha disj ren t).
 Proof.
-  soterm_ind t as [ v ts ind | op lbt ind ] Case; simpl; introv.
+  soterm_ind t as [ v ts ind | | op lbt ind ] Case; simpl; introv; tcsp.
 
   - Case "sovar".
     boolvar; subst; allsimpl; allrw @wf_sovar; allsimpl; tcsp.
@@ -1810,7 +1848,7 @@ Lemma wf_soterm_so_change_bvars_alpha {o} :
   forall (t : @SOTerm o) disj ren,
     wf_soterm t <=> wf_soterm (so_change_bvars_alpha disj ren t).
 Proof.
-  soterm_ind t as [ v ts ind | op lbt ind ] Case; simpl; introv.
+  soterm_ind t as [ v ts ind | | op lbt ind ] Case; simpl; introv; tcsp.
 
   - Case "sovar".
     split; intro k; apply wf_sovar; allsimpl; introv i; tcsp.
@@ -1903,7 +1941,7 @@ Lemma sovars2vars_so_free_vars_subvars_all_fo_vars {o} :
   forall (t : @SOTerm o),
     subvars (sovars2vars (so_free_vars t)) (all_fo_vars t).
 Proof.
-  soterm_ind t as [ v ts ind | op lbt ind ] Case; simpl; introv.
+  soterm_ind t as [ v ts ind | | op lbt ind ] Case; simpl; introv; tcsp.
 
   - Case "sovar".
     apply subvars_cons_lr.
@@ -2041,7 +2079,7 @@ Lemma so_free_vars_so_change_bvars_alpha {o} :
     so_free_vars (so_change_bvars_alpha disj ren t)
     = map (rename_sovar ren) (so_free_vars t).
 Proof.
-  soterm_ind t as [ v ts ind | op lbt ind ] Case; simpl; introv.
+  soterm_ind t as [ v ts ind | | op lbt ind ] Case; simpl; introv; tcsp.
 
   - Case "sovar".
     apply eq_cons.
@@ -2133,7 +2171,7 @@ Lemma so_free_vars_fo_change_bvars_alpha {o} :
     so_free_vars (fo_change_bvars_alpha disj ren t)
     = map (rename_sovar (foren2soren ren)) (so_free_vars t).
 Proof.
-  soterm_ind t as [ v ts ind | op lbt ind ] Case; simpl; introv.
+  soterm_ind t as [ v ts ind | | op lbt ind ] Case; simpl; introv; tcsp.
 
   - Case "sovar".
     boolvar; subst; allsimpl.
