computation/computation_preserve3.v
@@ -2,6 +2,7 @@
 
   Copyright 2014 Cornell University
   Copyright 2015 Cornell University
+  Copyright 2016 Cornell University
 
   This file is part of VPrl (the Verified Nuprl project).
 
@@ -19,7 +20,10 @@
   along with VPrl.  Ifnot, see <http://www.gnu.org/licenses/>.
 
 
-  Website: http://nuprl.org/html/verification/
+  Websites: http://nuprl.org/html/verification/
+            http://nuprl.org/html/Nuprl2Coq
+            https://github.com/vrahli/NuprlInCoq
+
   Authors: Abhishek Anand & Vincent Rahli
 
 *)
@@ -754,7 +758,8 @@ Lemma get_utokens_so_subset_get_cutokens_so {o} :
   forall (t : @SOTerm o),
     subseto (get_utokens_so t) (get_cutokens_so t).
 Proof.
-  soterm_ind1s t as [v ts ind|op bs ind] Case; simpl.
+  soterm_ind1s t as [v ts ind | |op bs ind] Case; simpl;
+  try (complete (eauto 3 with slow)).
 
   - Case "sovar".
     eapply subseto_oeqset;[|apply oeqset_sym;apply oeqset_oappl_OLL].
