continuity/continuity_defs.v
@@ -1,6 +1,8 @@
 (*
 
   Copyright 2014 Cornell University
+  Copyright 2015 Cornell University
+  Copyright 2016 Cornell University
 
   This file is part of VPrl (the Verified Nuprl project).
 
@@ -15,11 +17,14 @@
   GNU General Public License for more details.
 
   You should have received a copy of the GNU General Public License
-  along with VPrl.  Ifnot, see <http://www.gnu.org/licenses/>.
+  along with VPrl.  If not, see <http://www.gnu.org/licenses/>.
 
 
-  Website: http://nuprl.org/html/verification/
-  Authors: Abhishek Anand & Vincent Rahli
+  Websites: http://nuprl.org/html/verification/
+            http://nuprl.org/html/Nuprl2Coq
+            https://github.com/vrahli/NuprlInCoq
+
+  Authors: Vincent Rahli
 
 *)
 
@@ -690,7 +695,7 @@ Lemma all_fo_vars_eqvars {o} :
       (all_fo_vars t)
       (fo_bound_vars t ++ sovars2vars (so_free_vars t)).
 Proof.
-  soterm_ind t as [v ts ind|op bs ind] Case; simpl.
+  soterm_ind t as [v ts ind| |op bs ind] Case; simpl; auto.
 
   - Case "sovar".
     eapply eqvars_trans;[|apply eqvars_move_around].
@@ -3014,3 +3019,10 @@ Proof.
   introv i; repndors; cpx.
   apply alpha_eq_bterm_congr; auto.
 Qed.
+
+
+(*
+*** Local Variables:
+*** coq-load-path: ("." "../util/" "../terms/" "../computation/")
+*** End:
+*)
